erasure/theories/EWcbvEvalCstrsAsBlocksInd.v
@@ -517,6 +517,7 @@ Proof.
     split; intros; rtoProp; intuition auto; solve_all.
   - red.
     move=> hascase n ci discr brs. simpl.
+    rewrite /wf_brs.
     destruct lookup_inductive eqn:hl => /= //.
     intros; rtoProp; intuition auto; solve_all.
   - red. simpl. move=> hasproj n p discr wf discr' wf'.
